% !TEX TS-program = pdflatex
% !TEX encoding = UTF-8 Unicode

% This is a simple template for a LaTeX document using the "article" class.
% See "book", "report", "letter" for other types of document.

\documentclass[11pt]{article} % use larger type; default would be 10pt

\usepackage{amsmath}
\usepackage{amsfonts}
\usepackage[utf8]{inputenc} % set input encoding (not needed with XeLaTeX)


%%% END Article customizations

%%% The "real" document content comes below...

\title{Deriving the Distribution of the t Statistic}
\author{Ryan Lafferty}
%\date{} % Activate to display a given date or no date (if empty),
         % otherwise the current date is printed 

\begin{document}
\maketitle

%\subsection*{Finding the Distribution of t}
Let $X_1, ..., X_n$ be a sample from $N(\mu, \sigma^2)$ where $\sigma^2>0$ and $\mu\in\mathbb{R}$ and let $\mu_0$ be a fixed real number. We define the statistic $$t = \frac{\sqrt{n}(\bar{X} - \mu_0)}{s},$$ where $\bar{X} = \frac{1}{n}\sum_{i=1}^n X_i$ and $s^2 = \frac{1}{n-1} \sum_{i=1}^n (X_i - \bar{X})^2$. 

Recall that $Z = \frac{\sqrt{n}(\bar{X}-\mu)}{\sigma}$ has a standard normal distribution and that $W = \frac{(n-1)s^2}{\sigma^2}$ has a $\chi^2$ distribution with $n-1$ degrees of freedom. We have that 
\begin{align*}
t &= \frac{\sqrt{n}(\bar{X} - \mu_0)}{s}\\
& = \frac{\sqrt{n}(\bar{X} - \mu + \mu - \mu_0)/\sigma}{s/\sigma}\\
 & = \frac{Z + \frac{\sqrt{n}(\mu-\mu_0)}{\sigma}}{\sqrt{\frac{W}{n-1}}}
\end{align*}

Let $U_1 = Z + \frac{\sqrt{n}(\mu-\mu_0)}{\sigma}$ and let $U_2 = W$. Note that from the properties of the normal distribution, we know that $U_1$ and $U_2$ are independent. We will make the following transformation of variables: 
\begin{align*}
V_1 & = t =  (n-1)^{\frac{1}2} U_1 U_2^{-\frac{1}2}\\
V_2 & = U_2
\end{align*} 

The inverse transformation is given by:
\begin{align*}
U_1 &= (n-1)^{-\frac{1}2}V_1 V_2^{\frac{1}2} \\
U_2 &= V_2
\end{align*}

Next we need to compute the Jacobian. Since $\frac{\partial U_2}{\partial V_1} = 0$, the Jacobian is just 
$$J = \left|\frac{\partial U_1}{\partial V_1}\frac{\partial U_2}{\partial V_2 }\right| = (n-1)^{-\frac{1}2} V_2^{\frac{1}2}.$$

Since $Z$ is standard normal and $U_1$ is equal to $Z +  \frac{\sqrt{n}(\mu-\mu_0)}{\sigma}$, we have that $U_1 \sim N( \frac{\sqrt{n}(\mu-\mu_0)}{\sigma}, 1)$. Furthermore, $U_2 = W$ has a $\chi^2_{n-1}$ distribution and is independent of $U_1$. Therefore, we can easily give the joint pdf of $U_1$ and $U_2$ as follows: 
\begin{align*}
f_{U_1 U_2} (u_1, u_2) &= \left(\frac{1}{(2\pi)^{\frac{1}2}}e^{-\frac{1}{2} (u_1 - \frac{\sqrt{n}(\mu-\mu_0)}{\sigma})^2}\right)\left(\frac{1}{2^{\frac{n-1}2} \Gamma(\frac{n-1}2)}u_2^{\frac{n-1}{2} -1}e^{-\frac{u_2}2}\right)\\
&= \frac{1}{(2\pi)^{\frac{1}2}}\frac{1}{2^{\frac{n-1}2} \Gamma(\frac{n-1}2)}u_2^{\frac{n-1}{2} -1}e^{-\frac{u_2}2}e^{-\frac{1}{2} (u_1 - \frac{\sqrt{n}(\mu-\mu_0)}{\sigma})^2}\\
&= \frac{1}{\pi^{\frac{1}2} 2^{\frac{n}2} \Gamma(\frac{n-1}2)}u_2^{\frac{n-1}{2} -1}e^{-\frac{u_2}2-\frac{1}{2} (u_1 - \frac{\sqrt{n}(\mu-\mu_0)}{\sigma})^2}\\
& = C u_2^ k e^{-\frac{1}{2}u_2 - \frac{1}2 u_1^2 + \alpha u_1 - \frac{ \alpha^2}{2}},
\end{align*}
where $C =\frac{1}{\pi^{\frac{1}2} 2^{\frac{n}2} \Gamma(\frac{n-1}2)}$, $k = \frac{n-1}{2} -1$, and $\alpha = \frac{\sqrt{n}(\mu-\mu_0)}{\sigma}$. 

Thus, applying the change of variables formula yields: 
\begin{align*}
f_{V_1 V_2} (v_1, v_2)  & = C v_2^ k e^{-\frac{1}{2}v_2 - \frac{1}2 \frac{1}{n-1} v_2 v_1^2 + \alpha \frac{1}{\sqrt{n-1}}v_2^{\frac{1}2} v_1 - \frac{ \alpha^2}{2}}J\\
& = C^* v_2^ k e^{-\frac{1}{2}v_2 - \frac{1}2 \frac{1}{n-1} v_2 v_1^2 + \alpha \frac{1}{\sqrt{n-1}}v_2^{\frac{1}{2} v_1}{2}}v_2^{\frac{1}2}\\
& = C^* v_2^ {k+\frac{1}2} e^{-\frac{1}{2}(1+ \frac{1}{n-1}v_1^2  )v_2 + \alpha \frac{1}{\sqrt{n-1}}v_2^{\frac{1}2} v_1 }\\
\end{align*}
where $C^* = \frac{e^{ - \frac{ \alpha^2}2}}{\sqrt{n-1}}C$. We want to find the marginal pdf $$f_{V_1}(v_1) = C^* \int_{0}^{\infty}v_2^ {k+\frac{1}2} e^{-\frac{1}{2}(1+ \frac{1}{n-1}v_1^2  )v_2 + \alpha \frac{1}{\sqrt{n-1}}v_2^{\frac{1}2} v_1 } dv_2.$$
Let us first make the substitution $s = \sqrt{v_2},$ which we are free to do since $v_2$ is always non-negative. Differentiating the expression $s^2 = v_2$ gives $$2s ds = dv_2.$$ so that now we have 
\begin{align*}
f_{V_1}(v_1) &= C^* \int_{0}^{\infty}s^ {2k+1} e^{-\frac{1}{2}(1+ \frac{1}{n-1}v_1^2  )s^2 + \frac{\alpha}{\sqrt{n-1}} v_1 s } (2s) ds\\
&= 2C^* \int_{0}^{\infty}s^ {2k+2} e^{-\frac{1}{2}(1+ \frac{1}{n-1}v_1^2  )s^2 + \frac{\alpha}{\sqrt{n-1}} v_1 s } ds\\
\end{align*}
The expression $-\frac{1}{2}(1+ \frac{1}{n-1}v_1^2  )s^2 + \frac{\alpha}{\sqrt{n-1}} v_1 s $ can be written in the form $a (s - b)^2 + c$ since it is a quadratic polynomial. In that case, we have $a = -\frac{1}{2}(1+ \frac{1}{n-1}v_1^2  )$, $-2 a b = \frac{\alpha}{\sqrt{n-1}} v_1$, and $c =- a b^2$.  Solving for $b$ and $c$, we have 
\begin{align*}
a &= -\frac{1}{2}(1+ \frac{1}{n-1}v_1^2  )\\
b & =  \frac{\alpha}{\sqrt{n-1}}\frac{ v_1}{(1+ \frac{1}{n-1}v_1^2  )} \\
c & = -\frac{1}{2}\frac{\alpha^2}{n-1}\frac{ v_1^2}{(1+ \frac{1}{n-1}v_1^2  )}
\end{align*}

The integral becomes 
\begin{align*}
f_{V_1}(v_1) &= 2C^* e^c \int_{0}^{\infty}s^ {2k+2} e^{a (s - b)^2 } ds\\
\end{align*}

Let $r = -a(s - b)^2$ with $dr = -2a s \: ds $. We have $s = b + \sqrt{-\frac{r}{a}}$, which is a real number since $a<0$. In this case $r$ will run from $-ab^2 = c$ to $-\infty$. We can write
\begin{align*}
f_{V_1}(v_1) &= - \frac{C^* e^c}{a} \int_{c}^{-\infty}\left(b + \sqrt{-\frac{r}{a}}\right)^ {2k+1} e^{-r } dr \\
 &=  \frac{C^* e^c}{a} \int_{-\infty}^{c}\left(b + \sqrt{-\frac{r}{a}}\right)^ {2k+1} e^{-r } dr \\
 &=  \frac{C^* e^c}{a} \sum_{i = 0}^{2k + 1} {2k + 1 \choose i}b^{2k+1-i}\int_{-\infty}^{c}\left(\sqrt{-\frac{r}{a}}\right)^ {i} e^{-r } dr \\
 &=  \frac{C^* e^c}{a} \sum_{i = 0}^{2k + 1} {2k + 1 \choose i}\frac{b^{2k+1-i}}{(-a)^{\frac{i}2}}\int_{-\infty}^{c}r^{\frac{i}2} e^{-r } dr \\
 &=  \frac{C^* e^c}{a} \sum_{i = 0}^{2k + 1} {2k + 1 \choose i}\frac{b^{2k+1-i}}{(-a)^{\frac{i}2}}\int_{-\infty}^{c}r^{\frac{i}2} e^{-r } dr \\
\end{align*}

\end{document}
